make base version of BigInt working with lean frontend

test/lean/Proofs.lean
@@ -1,44 +1,425 @@
-import Test.MyFuns
+import Test.Funs
+import Base
 
 open Primitives
 open Result
-open test
+-- open test
 
 namespace test
 
-namespace arithmetics
+namespace biginteger
 
-def BigInt.valImpl (l : List U64) : Int :=
+-- namespace arithmetics
+
+attribute [-simp] Bool.exists_bool
+
+def valImpl (l : List U64) : Int :=
   match l with
   | a::b => a.val + (valImpl b) * (2 ^ 64)
   | [] => 0
 
-def BigInt.val {N : Usize} (x : BigInt N) : Int := valImpl x.num.val
+lemma valImpl_ge_zero (l : List U64) : valImpl l ≥ 0 := by
+  unfold valImpl
+  match l with
+  | a::b => {
+    have ha : 0 ≤ a.val := by scalar_tac
+    have hb : 0 ≤ valImpl b * 2 ^ 64 := by simp[valImpl_ge_zero]
+    have hc := Int.add_le_add ha hb
+    simp at hc
+    simp [*]
+  }
+  | [] => simp
 
-def BigInt.max_value (N : Usize) : Int := (U64.max + 1) ^ (Int.toNat N.val) - 1
+@[simp]
+lemma tmp : Inhabited U64 := by
+  constructor
+  apply 0#u64
+
+-- Biggest part by Son Ho
+lemma BigInt.update_eq (l : List U64) (i : Int) (x : U64)
+  (h0 : 0 ≤ i) (h1 : i < l.len) :
+  valImpl (l.update i x) = valImpl l + (x - l.index i) * ((2 ^ 64) ^ i.toNat) := by
+  match l with
+  | [] =>
+    -- Contradiction: 0 ≤ i ∧ i < 0
+    simp at h1
+    scalar_tac
+  | h :: tl =>
+    simp at h1
+    if i = 0 then
+      simp [*] -- By writing [*] I'm using the hypothesis i = 0
+      unfold valImpl
+      scalar_tac
+    else
+      have hnz : i ≠ 0 := by scalar_tac
+      -- This uses update_nzero_cons and index_nzero_cons
+      simp only [h1, hnz, ne_eq, not_false_eq_true, List.update_nzero_cons, List.index_nzero_cons] -- By writing [*] I'm using the hypothesis i ≠ 0
+      unfold valImpl
+      -- Recursive call
+      have heq := update_eq tl (i - 1) x (by scalar_tac) (by scalar_tac)
+      rw [heq]
+      rw [add_mul]
+      simp only [Int.pred_toNat]
+      have hexpr : ((2: Int) ^ 64) ^ (Int.toNat i - 1) * 2 ^ 64 = (2 ^ 64) ^ Int.toNat i := by {
+        rw [←pow_mul]
+        rw [←pow_add]
+        rw [←pow_mul]
+        rw [Nat.mul_sub_left_distrib]
+        rw [←Nat.sub_add_comm]
+        simp [*]
+        have hgone : i ≥ 1 := by scalar_tac
+        simp [hgone, *]
+      }
+      simp only [mul_assoc]
+      rw [hexpr]
+      simp [add_assoc]
+
+
+@[simp] lemma BigInt.len_spec
+  (N : Usize) (self : biginteger.BigInt N) :
+  (self.val).len = N.val := by
+  have h := self.property
+  rw [List.len_eq_length]
+  apply h
+
+def BigInt.val {N : Usize} (x : biginteger.BigInt N) : Int := valImpl (Array.v x)
+
+def BigInt.mod_value (n : Int) : Int := (U64.max + 1) ^ (Int.toNat n)
+
+def BigInt.max_value (n : Int) : Int := BigInt.mod_value n - 1
+
+lemma BigInt.mod_value_add_one (n : Int) (hn : 0 ≤ n) : BigInt.mod_value n * (2 ^ 64) = BigInt.mod_value (n + 1) := by
+  rw [BigInt.mod_value]
+  rw [BigInt.mod_value]
+  rw [U64.max]
+  simp
+  -- rw [mul_comm]
+  rw [←pow_succ]
+  -- simp []
+  have hf := Int.toNat_add_nat hn 1
+  rw [←hf]
+  simp
+
+lemma valImpl_lt_mod (l : List U64) : valImpl l < BigInt.mod_value l.len := by
+  unfold valImpl
+  match h : l with
+  | a::b => {
+    simp only [List.len_cons, gt_iff_lt]
+    have ha := valImpl_lt_mod b
+    have hb : a.val < 2 ^ 64 := by scalar_tac
+    have hc := Int.le_sub_one_of_lt ha
+    have hd : 1 + b.len = b.len + 1 := by scalar_tac
+    have hf : (0 : Int) ≤ 2 ^ 64 := by simp 
+    have hg := Int.mul_le_mul_of_nonneg_right hc hf
+    simp only [Int.sub_mul] at hg
+    simp only [one_mul] at hg
+    have hh := add_lt_add_of_le_of_lt hg hb
+    simp only [sub_add_cancel] at hh
+    rw [Int.add_comm] at hh
+    rw [hd]
+    rw [←BigInt.mod_value_add_one]
+    simp only [hh]
+    scalar_tac
+  }
+  | [] => {
+    simp
+    unfold BigInt.mod_value
+    simp
+  }
+
+
+lemma BigInt.val_lt_mod (N : Usize) (bn : Array U64 N) : valImpl bn.val < BigInt.mod_value N.val := by
+  have hi := valImpl_lt_mod bn.val
+  have he := bn.property
+  simp [*, List.len_eq_length] at hi
+  simp [*]
 
 theorem adc_for_add_with_carry_spec (a : U64) (b : U64) (carry : U8) :
-  match adc_for_add_with_carry a b carry with
-  | ret new_carry => new_carry = (a.val + b.val + carry.val) / (2 ^ 64)
-  | _ => ⊥
-  := by sorry
-
-theorem adc_for_add_with_carry_back_spec (a : U64) (b : U64) (carry : U8) :
-  ∃ new_a, adc_for_add_with_carry_back a b carry = .ret new_a ∧
-  new_a = (a.val + b.val + carry.val) * 2 ^ 64 := by sorry
+  ∃ new_carry r, biginteger.arithmetic.adc_for_add_with_carry a b carry = .ok (new_carry, r) ∧ 
+  new_carry = (a.val + b.val + carry.val) / (2 ^ 64) ∧
+  r = (a.val + b.val + carry.val) % 2 ^ 64 := by sorry
 
 
-lemma add_with_carry_overflow : 
-  ∀ (N : Usize) (self : arithmetics.BigInt N) (other : arithmetics.BigInt N),
-  ∃ b, arithmetics.BigInt.add_with_carry N self other = .ret b ∧
-  ¬b ↔ self.val + other.val ≤ BigInt.max_value N := sorry
-    -- by unfold arithmetics.BigInt.add_with_carry
+lemma BigInt.ha_0_val (N: Usize) (bi : Array U64 N) : N = 0#usize → valImpl bi.val = 0 := 
+by {
+      unfold valImpl;
+      intro hN;
+      have h := bi.property;
+      match hq0 : bi.val with
+        | [] => scalar_tac;
+        | hd :: tl => {
+            simp [BigInt.len_spec, hN, List.len_eq_length, *] at h; scalar_tac;
+        }
+  }
+
+-- lemma BigInt.h_1_val (N: Usize) (bi : BigInt N) : N = 1#usize → valImpl (Array.v bi) = (Array.v bi).index 0#usize.val  := 
+-- by {
+--         simp [BigInt.val]; 
+--         unfold valImpl;
+--         have h := BigInt.len_spec N bi;
+--         match hq0 : bi.val with
+--         | [] => simp [List.len_nil, Usize.ofInt_val_eq, hq0] at h; scalar_tac;
+--         | hd :: tl => {
+--           simp []
+--           unfold valImpl
+--           match hq1 : tl with
+--           | [] => simp [];
+--           | hd::tl2 => simp [*, List.len_eq_length] at h; scalar_tac;
+--         }
+--       }
+
+lemma BigInt.slice_eq (l : List U64) (i : Int) (N : Int)
+  (h0 : 0 ≤ i) (h1 : i < N) (h2 : N ≤ l.len) :
+  valImpl (l.slice i N) = (2 ^ 64) * valImpl (l.slice (i + 1) N) + (l.index i) := by
+    match l with
+    | h::tl => {
+      if hi : i = 0
+      then {
+        rw [hi]
+        simp only [zero_add, ne_eq, zero_ne_one, not_false_eq_true, neq_imp,
+          List.slice_nzero_cons, sub_self, List.index_zero_cons]
+        rw [List.slice]
+        simp only [sub_zero, List.idrop_zero]
+        rw [List.itake]
+        have h3 := lt_of_le_of_lt h0 h1
+        have h4 := ne_of_lt h3
+        simp only [h4, not_false_eq_true, neq_imp, ↓reduceIte]
+        rw [valImpl]
+        rw [add_comm]
+        rw [mul_comm]
+        rw [List.slice]
+        simp
+      }
+      else {
+        have hi1 : i + 1 ≠ 0 := by scalar_tac
+        simp only [ne_eq, not_false_eq_true, List.slice_nzero_cons, List.index_nzero_cons, hi, hi1]
+        rw [BigInt.slice_eq]
+        simp
+        scalar_tac
+        scalar_tac
+        simp [*] at h2
+        rw [add_comm] at h2
+        simp [*]
+      }
+    }
+    | [] => {
+      simp at h2
+      have h3 := lt_of_le_of_lt h0 h1
+      have h4 := not_le_of_lt h3
+      simp [h2] at h4
+    }
+
+lemma BigInt.mod_value_eq (n : Int) : BigInt.mod_value n = (2 ^ 64) ^ n.toNat := by
+  rw [BigInt.mod_value]
+  rw [U64.max]
+  simp
+  
+lemma add_with_carry_loop_correct :
+  ∀ (N : Usize) (self : Array U64 N) (other : Array U64 N) (carry : U8) (i : Usize) (h : i ≤ N),
+  ∃ b v, biginteger.BigIntegertestbigintegerBigIntN.add_with_carry_loop N self other carry i = .ok (b, v) ∧
+  (valImpl v.v) = (valImpl self.val + (BigInt.mod_value i.val) * (valImpl (other.val.slice i.val N.val) + carry.val)) % (BigInt.mod_value N.val) := by
+    intro N
+    intro self other
+    intro carry
+    intro i
+    intro h
+    rw [biginteger.BigIntegertestbigintegerBigIntN.add_with_carry_loop]
+    if hind : (N.val - i.val).toNat = 0 then
+      have hieqN : i = N := by {
+        simp only [Int.toNat_eq_zero, tsub_le_iff_right, zero_add] at hind; 
+        simp [Scalar.le_equiv] at h
+        scalar_tac
+      }
+      simp only [hieqN, Scalar.lt_equiv, lt_self_iff_false, ↓reduceIte, ok.injEq, Prod.mk.injEq,
+        Int.add_mul_emod_self_left]
+      exists (carry != 0#u8), self
+      have modh := Int.emod_eq_of_lt (valImpl_ge_zero self.val) (BigInt.val_lt_mod N self)
+      simp only [and_self, true_and]
+      simp [*]
+    else
+      have hiltN : i < N := by {
+        simp only [Int.toNat_eq_zero, tsub_le_iff_right, zero_add, not_le] at hind 
+        simp [Scalar.lt_equiv]
+        scalar_tac
+      }
+      simp only [hiltN, lt_self_iff_false, ↓reduceIte]
+
+      progress with Array.index_mut_usize_spec as ⟨ i1, hi1, hi1d, hi1a ⟩
+      progress with Array.index_usize_spec as ⟨ i2, hi2 ⟩
+      progress with adc_for_add_with_carry_spec as ⟨ i3, hi3, hi3d, hi3a ⟩
+      progress as ⟨ w1, hw1 ⟩
+      simp only [hi1a, hi3a]
+      progress with Array.update_usize_spec as ⟨ a1, ha1 ⟩
+      progress with add_with_carry_loop_correct as ⟨ i4, hi4, hi4d ⟩
+      . scalar_tac
+      exists i4, hi4
+      simp only [true_and]
+      rw [hi4d]
+      -- rw [hi3d]
+      rw [ha1]
+      -- rw [hi1d]
+      -- rw [hi2]
+      rw [BigInt.update_eq]
+      -- have hEliminSelf {m : Int} {k : Int} := @Int.emod_add_cancel_left m (BigInt.mod_value N) k (valImpl self.val)
+      rw [add_assoc]
+      rw [Int.emod_add_cancel_left]
+      have hOldSlice := BigInt.slice_eq other.val i.val N.val (by scalar_tac) (by scalar_tac) (by scalar_tac)
+      -- rw [BigInt.slice_eq]
+
+      rw [hOldSlice]
+
+      rw [hw1]
+      -- rw [hi3a]
+      -- rw [hi2]
+      -- rw [hi3d]
+      simp only [Scalar.ofInt_val_eq]
+      simp only [Int.mul_add]
+      rw [←Int.mul_assoc]
+      rw [BigInt.mod_value_add_one]
+      rw [Int.add_comm]
+      rw [Int.add_assoc]
+      rw [Int.add_assoc]
+      rw [Int.emod_add_cancel_left]
+      rw [←BigInt.mod_value_add_one]
+      rw [←BigInt.mod_value_eq]
+      rw [Int.mul_assoc]
+      have htmp : (hi3.val - ((self.val).index i.val).val) * BigInt.mod_value i.val = BigInt.mod_value i.val * (hi3.val - ((self.val).index i.val).val) := by simp [Int.mul_comm]
+      rw [htmp]
+      rw [←Int.mul_add]
+      rw [←Int.mul_add]
+      rw [hi3d]
+      rw [hi3a]
+      rw [←add_sub_assoc]
+      rw [Int.ediv_add_emod]
+      have htmp1 : i1.val + i2.val + carry.val = i2.val + carry.val + i1.val := by scalar_tac
+      rw [htmp1]
+      rw [hi1d]
+      rw [add_sub_assoc]
+      simp only [sub_self, add_zero]
+
+      rw [hi2]
+      --------------------------------------------
+
+      scalar_tac
+      scalar_tac
+      scalar_tac
+      scalar_tac
+termination_by (N.val - i.val).toNat
+decreasing_by
+  simp_wf
+  rw [hw1]
+  simp [sub_add_eq_sub_sub, *]
+  -- sorry
+  -- scalar_decr_tac
+  -- scalar_tac
+  apply Arith.to_int_sub_to_nat_lt
+  simp [sub_one_lt, Int.toNat_sub, Int.toNat_sub_of_le, h, *]
+  scalar_tac
+  simp [sub_one_lt, *]
+
+
+lemma full_itake (l : List α) (N: Int) (h : N = l.len): List.itake N l = l := by
+  unfold List.itake;
+  match hl : l with
+  | [] => simp [hl];
+  | hs::tl => {
+    if hn : N = 0 then
+      simp at h;
+      scalar_tac;
+    else
+      simp only [hn, not_false_eq_true, neq_imp, ↓reduceIte, List.cons.injEq, true_and];
+      simp [full_itake, *]
+  }
+
+lemma full_slice (l : List α) (N: Int) (h : N = l.len): List.slice 0 N l = l := by
+  unfold List.slice
+  simp only [sub_zero, List.idrop_zero]
+  simp only [full_itake, h]
+
+-- lemma inductive_overflow:
+-- ∀ (N:Usize) (self : BigInt N) (other : BigInt N)(b1:Bool)(val1: BigInt (N))
+-- (h1:N ≥ 1#usize )(h2: add_with_carry N self other = .ret (b1, val1)), (∃ (M:Usize) (self_reduit : arithmetics.BigInt (M)) (other_reduit : arithmetics.BigInt (M)) 
+-- (self_val:U64) (other_val:U64)  (val2:arithmetics.BigInt (M))
+--  (b2:Bool), N-1#usize=ret M ∧  self.num.val=self_val::self_reduit.num.val ∧ other.num.val=other_val::other_reduit.num.val
+-- ∧arithmetics.BigInt.add_with_carry M self_reduit other_reduit = .ret (b2, val2) ∧ 
+-- ((b1=true) ↔ (self_val+other_val ≥ U64.max ∨ (self_val+other_val = U64.max-1 ∧ b2)))):=
+-- sorry
+
+-- lemma inductive_addition:
+-- ∀ (N:Usize) (self : arithmetics.BigInt N) (other : arithmetics.BigInt N)(M:Usize)
+-- (self_val:U64)(other_val:U64)(h1:N ≥ 1#usize )(h2:N-1#usize=ret M)
+-- (h3:∃self_reduit : arithmetics.BigInt (M),self.num.val=self_val::self_reduit.num.val)
+-- (h4:∃other_reduit : arithmetics.BigInt (M),other.num.val=other_val::other_reduit.num.val),
+-- self_val+other_val≤U64.max-2 → self.val+other.val ≤ BigInt.max_value N:=
+-- by sorry
+
+-- def toInt : U8 →  ℤ
+-- | ⟨val, _,_⟩ => val
+
+-- lemma add_with_carry_loop_overflow_correct
+--   (N : Usize) (self : Array U64 N) (other : Array U64 N) (carry : U8) (i : Usize)
+--   (h : i ≤ N) (hc : toInt carry ≤ 1) :
+--   ∃ b v, arithmetics.BigInt.add_with_carry_loop N self other carry i = .ret (b, v) ∧
+--   (b ↔ valImpl self.val + valImpl other.val + carry.val  > BigInt.max_value N) := by
+--   sorry
+
+def bool_to_int (b:Bool) := if b then 0 else (1 : Int)
+
+lemma add_with_carry_spec (N : Usize) (self : BigInt N) (other : BigInt N) :
+  ∃ b v, biginteger.BigIntegertestbigintegerBigIntN.add_with_carry N self other = .ok (b, v) ∧
+  (bool_to_int b) * (BigInt.mod_value N.val) + v.val = self.val + other.val
+  := by
+  sorry
+
+-- lemma add_with_carry_overflow [Inhabited U64] : 
+--   ∀ (N : Usize) (self : BigInt N) (other : BigInt N),
+--   ∃ b val, biginteger.BigIntegertestbigintegerBigIntN.add_with_carry N self other = .ret (b, val) ∧
+--   (¬b ↔ self.val + other.val ≤ BigInt.max_value N) :=
+-- by
+--   intro N₁
+--   intro s₁ o₁
+--   simp only [biginteger.BigIntegertestbigintegerBigIntN.add_with_carry]
+--   progress with add_with_carry_loop_overflow_correct as ⟨ i, hi, hid ⟩
+--   . scalar_tac
+--   rw [toInt]
+--   simp
+--   exists i,{num:=hi}
+--   simp
+--   apply Iff.intro
+--   intro h₀
+--   rw [h₀] at hid
+--   simp at hid
+--   rw [BigInt.val]
+--   exact hid
+--   intro h₁
+--   simp [BigInt.val] at h₁
+--   contrapose! h₁
+--   simp at h₁
+--   rw [h₁] at hid
+--   simp at hid
+--   exact hid
 
 lemma add_with_carry_correct :
-  ∀ (N : Usize) (self : arithmetics.BigInt N) (other : arithmetics.BigInt N),
-  ∃ v, arithmetics.BigInt.add_with_carry_back N self other = .ret v ∧
-  v.val = (self.val + other.val) % (BigInt.max_value N) := sorry
+  ∀ (N : Usize) (self : BigInt N) (other : BigInt N),
+  ∃ b v, biginteger.BigIntegertestbigintegerBigIntN.add_with_carry N self other = .ok (b, v) ∧
+  v.val = (self.val + other.val) % (BigInt.mod_value N.val) := by
+    intro N
+    intro self other
+    simp only [biginteger.BigIntegertestbigintegerBigIntN.add_with_carry]
+    progress with add_with_carry_loop_correct as ⟨ i, hi, hid ⟩
+    . scalar_tac
+    exists i, hi
+    simp only [true_and] 
+    unfold BigInt.mod_value at hid
+    simp only [Scalar.ofInt_val_eq, Int.toNat_zero, pow_zero, one_mul] at hid
+    have other_full_slice : List.slice 0 N.val other.v = other.v := by simp only [BigInt.len_spec, full_slice]
+    simp only [other_full_slice] at hid 
+    unfold BigInt.val
+    unfold BigInt.mod_value
+    simp [*]
 
-end arithmetics
+-- end arithmetics
+
+end biginteger
 
 end test
